common/spec/GC.Spec.Object.fst
@@ -22,10 +22,6 @@ open GC.Lib.Header
 /// Tag Constants
 /// ---------------------------------------------------------------------------
 
-let closure_tag : U64.t = 247UL
-let infix_tag : U64.t = 249UL
-let no_scan_tag : U64.t = 251UL
-
 let no_scan_tag_val () : Lemma (no_scan_tag == U64.uint_to_t 251) = ()
 let infix_tag_val () : Lemma (infix_tag == U64.uint_to_t 249) = ()
 
