generational/spec/GC.Gen.CombinedGraph.fsti
@@ -198,6 +198,7 @@ val minor_field_edge_intro (ms: minor_state) (major: heap)
   (src: U64.t) (i: nat) (dst: combined_vertex)
   : Lemma (requires Seq.mem src (minor_objects ms) /\
                     i < minor_wosize ms src /\
+                    ~(minor_is_no_scan ms src) /\
                     classify_minor_field ms major (minor_read_field ms src i) == Some dst)
           (ensures mem_ce (MinorV src, dst) (build_combined_graph ms major))
 
@@ -235,6 +236,7 @@ val minor_edge_elim (ms: minor_state) (major: heap)
   (src: U64.t) (dst: combined_vertex)
   : Lemma (requires mem_ce (MinorV src, dst) (build_combined_graph ms major))
           (ensures Seq.mem src (minor_objects ms) /\
+                   ~(minor_is_no_scan ms src) /\
                    (exists (i: nat). i < minor_wosize ms src /\
                      classify_minor_field ms major (minor_read_field ms src i) == Some dst))
 
